WiP: trying to prove coherency and monotonicity

src/traversal/SimTravClosure.v
@@ -43,24 +43,62 @@ Module SimTravClosure.
   Definition Cclos (tc: trav_config) :=
     issued tc ∩₁ (is_rel lab) ∪₁ codom_rel (⦗covered tc ∪₁ issued tc ∩₁ is_rel lab⦘ ⨾ rmw).
   Definition Iclos (tc: trav_config) :=
-    (covered tc ∪₁ Cclos tc) ∩₁ W. 
+    (* (covered tc ∪₁ Cclos tc) ∩₁ W. *)
+    codom_rel (⦗covered tc⦘ ⨾ rmw). 
 
-  Lemma stc_alt_unfolded (tc: trav_config):
-    let (C, I) := tc in
-    let C' := I ∩₁ (is_rel lab) ∪₁ codom_rel (⦗C ∪₁ I ∩₁ is_rel lab⦘ ⨾ rmw) in
-    let I' := (C ∪₁ I ∩₁ (is_rel lab) ∪₁ codom_rel (⦗C ∪₁ I ∩₁ (is_rel lab)⦘ ⨾ rmw)) ∩₁ W in
-    sim_trav_closure tc = tc ⊔ (mkTC C' I'). 
+  Lemma codom_I_rmw_empty WF WFSC
+        (tc: trav_config) (COH: tc_coherent G sc tc):
+    codom_rel (⦗(issued tc) ∩₁ is_rel lab⦘ ⨾ rmw) ≡₁ ∅.
   Proof.
-    unfold sim_trav_closure. destruct tc as [C I]. simpl.
-    apply trav_config_eq_helper; simpl; basic_solver 10.
-  Qed.     
+    rewrite wf_rmwD; auto. repeat seq_rewrite <- id_inter.
+    forward eapply tc_I_in_W as IW; eauto.
+    { apply tc_coherent_implies_tc_coherent_alt; eauto. }
+    simpl in IW. split; [| basic_solver]. rewrite IW. type_solver.
+  Qed. 
 
-  Lemma stc_alt (tc: trav_config):
+  Lemma stc_alt WF WFSC
+        (tc: trav_config) (COH: tc_coherent G sc tc):
     sim_trav_closure tc = tc ⊔ (mkTC (Cclos tc) (Iclos tc)). 
   Proof.
+    forward eapply tc_coherent_implies_tc_coherent_alt as COH'; eauto. 
     unfold sim_trav_closure, Iclos, Cclos. destruct tc as [C I]. simpl.
-    apply trav_config_eq_helper; simpl; basic_solver 10. 
+    unfold trav_config_union. simpl. 
+    apply trav_config_eq_helper; simpl.
+    { basic_solver 10. }
+    rewrite !set_inter_union_l.
+    rewrite <- !set_unionA. apply set_equiv_union.
+    { split; [| basic_solver].
+      forward eapply tc_W_C_in_I as CI; eauto.         
+      simpl in CI. rewrite CI. basic_solver. }
+    rewrite id_union, !seq_union_l. rewrite codom_union, set_inter_union_l.  
+    split.
+    2: { rewrite wf_rmwD at 1; auto.
+         apply set_subset_union_r. left. basic_solver. }
+    apply set_subset_union_l. split; [basic_solver| ].
+    etransitivity; [| apply set_subset_empty_l].
+    forward eapply codom_I_rmw_empty as IW; eauto. simpl in IW.
+    rewrite IW. basic_solver 10. 
   Qed.
+
+  (* Lemma stc_alt_unfolded (tc: trav_config): *)
+  (*   let (C, I) := tc in *)
+  (*   let C' := I ∩₁ (is_rel lab) ∪₁ codom_rel (⦗C ∪₁ I ∩₁ is_rel lab⦘ ⨾ rmw) in *)
+  (*   let I' := (C ∪₁ I ∩₁ (is_rel lab) ∪₁ codom_rel (⦗C ∪₁ I ∩₁ (is_rel lab)⦘ ⨾ rmw)) ∩₁ W in *)
+  (*   sim_trav_closure tc = tc ⊔ (mkTC C' I').  *)
+  (* Proof. *)
+  (*   unfold sim_trav_closure. destruct tc as [C I]. simpl. *)
+  (*   apply trav_config_eq_helper; simpl; basic_solver 10. *)
+  (* Qed.      *)
+
+  (* Lemma stc_alt_unfolded (tc: trav_config): *)
+  (*   let (C, I) := tc in *)
+  (*   let C' := I ∩₁ (is_rel lab) ∪₁ codom_rel (⦗C ∪₁ I ∩₁ is_rel lab⦘ ⨾ rmw) in *)
+  (*   let I' := (C ∪₁ I ∩₁ (is_rel lab) ∪₁ codom_rel (⦗C ∪₁ I ∩₁ (is_rel lab)⦘ ⨾ rmw)) ∩₁ W in *)
+  (*   sim_trav_closure tc = tc ⊔ (mkTC C' I'). *)
+  (* Proof. *)
+  (*   unfold sim_trav_closure. destruct tc as [C I]. simpl. *)
+  (*   apply trav_config_eq_helper; simpl; basic_solver 10. *)
+  (* Qed. *)
 
   Lemma stc_tcu_distribute (tc1 tc2: trav_config):
     sim_trav_closure (tc1 ⊔ tc2) =
@@ -149,41 +187,163 @@ Module SimTravClosure.
     { destruct NEW. left. rewrite H0. left. apply COVEQ. basic_solver. }
     destruct NEW. right. rewrite H1. left. apply ISSEQ. basic_solver.
   Qed. 
-    
 
-
-  (* Lemma isim_trav_step_mon' thread *)
-  (*       (C1 I1 C2 I2 C' I' C'' I'': actid -> Prop) *)
-  (*       (STEP: isim_trav_step G sc thread (mkTC C1 I1) (mkTC C2 I2)) *)
-  (*       (MON_C: C' ⊆₁ C'') (MON_I: I' ⊆₁ I'') *)
-  (*       : *)
-  (*   (isim_trav_step G sc thread)^? (mkTC (C1 ∪₁ C') (I1 ∪₁ I')) *)
-  (*                  (mkTC (C2 ∪₁ C'') (I2 ∪₁ I'')). *)
+  (* Lemma isim_trav_step_mon_add_cov (e: actid) *)
+  (*       (C1 I1 C2 I2 C' I': actid -> Prop) *)
+  (*       (STEP: itrav_step G sc e {| covered := C1; issued := I2 |} *)
+  (*                         {| covered := C1 ∪₁ eq e; issued := I2 |}) *)
+  (*       (NCOVe: ~ (C1 ∪₁ C') e): *)
+  (* isim_trav_step G sc (tid e) {| covered := C1 ∪₁ C'; issued := I2 ∪₁ I' |} *)
+  (*                {| covered := C1 ∪₁ eq e ∪₁ C'; issued := I2 ∪₁ I' |}. *)
   (* Proof. *)
-  (*   inversion STEP; subst; simpl in *. *)
-  (*   { destruct (classic ((C1 ∪₁ C') f)). *)
-  (*     { left. apply trav_config_eq_helper; simpl. basic_solver. } *)
-  (*     right. *)
-  (*     assert (C1 ∪₁ eq f ∪₁ C' ≡₁ C1 ∪₁ C' ∪₁ eq f) as C_ALT by basic_solver. *)
-  (*     erewrite trav_config_eq_helper'; [| simpl; by apply C_ALT | reflexivity]. *)
-  (*     simpl. *)
-  (*     apply fence_trav_step; auto. simpl. *)
-  (*     erewrite trav_config_eq_helper'; [| simpl; by rewrite <- C_ALT | reflexivity]. *)
-  (*     simpl. *)
-  (*     eapply itrav_step_mon_ext with (C' := C') (I' := I') in TS as [? | ?]. *)
-  (*     2: { eapply itrav_step_eq; [| | by apply H0]; basic_solver. } *)
-  (*     inversion H0. destruct H. rewrite H2. basic_solver. } *)
-  (* Admitted. *)
-  
+  (*   assert (C1 ∪₁ eq e ∪₁ C' ≡₁ C1 ∪₁ C' ∪₁ eq e) as C_ALT by basic_solver.  *)
+  (*   erewrite trav_config_eq_helper'; [| simpl; by apply C_ALT | reflexivity]. *)
+  (*   simpl. *)
+
+    
+    
+  (*   apply fence_trav_step; auto. simpl. *)
+  (*   erewrite trav_config_eq_helper'; [| simpl; by rewrite <- C_ALT | reflexivity]. *)
+  (*   simpl. *)
+  (*   eapply itrav_step_mon_ext with (C' := C') (I' := I') in TS as [? | ?]. *)
+  (*   2: { eapply itrav_step_more; [reflexivity| .. | apply H0]. *)
+  (*        all: by apply same_tc_Symmetric. } *)
+  (*   inversion H0. destruct H. rewrite H2. basic_solver.      *)
+
+  (* Lemma stc_coherent (tc: trav_config) WF WFSC *)
+  (*       (COH: tc_coherent G sc tc): *)
+  (*   tc_coherent G sc (sim_trav_closure tc). *)
+  (* Proof. *)
+  (*   pose proof COH as COH'. red in COH'. desc.  *)
+  (*   rewrite stc_alt; auto. *)
+  (*   forward eapply codom_I_rmw_empty as CIR; eauto.  *)
+  (*   destruct tc as [C I] eqn:TC. simpl in *.  *)
+  (*   unfold trav_config_union. simpl. red. splits; simpl.  *)
+  (*   { etransitivity; [apply ICOV| ]. basic_solver. } *)
+  (*   { unfold Cclos, coverable. simpl.  *)
+
+  Lemma sb_invrmw_sbclos WF:
+    sb ⨾ rmw⁻¹ ⊆ sb^?.
+  Proof.
+    red. ins. destruct (classic (x = y)); [by left| ].
+    right. red in H. destruct H as [w [SB RMW]]. red in RMW.
+    forward eapply (wf_rmwi WF _ _ RMW) as [SByw IMMyw]. 
+    eapply sb_semi_total_r in SByw; eauto.
+    2: { eapply read_or_fence_is_not_init; eauto. left.
+         apply wf_rmwD, seq_eqv_lr in RMW; auto. by desc. }
+    des; auto. edestruct IMMyw; eauto. 
+  Qed. 
+    
+  (* Lemma sb_invrmw_sbclos_ext WF: *)
+  (*   sb ⨾ rmw⁻¹ ⊆ sb^? ⨾ ⦗W⦘ ⨾ sb^?. *)
+  (* Proof. *)
+  (*   red. ins. destruct (classic (x = y)). *)
+  (*   { subst. red in H. desc. red in H0.  *)
+  (*     apply seqA. red. exists z. split; [| basic_solver]. *)
+  (*     apply seq_eqv_r. split; [| basic_solver]. *)
+  (*   right. red in H. destruct H as [w [SB RMW]]. red in RMW. *)
+  (*   forward eapply (wf_rmwi WF _ _ RMW) as [SByw IMMyw].  *)
+  (*   eapply sb_semi_total_r in SByw; eauto. *)
+  (*   2: { eapply read_or_fence_is_not_init; eauto. left. *)
+  (*        apply wf_rmwD, seq_eqv_lr in RMW; auto. by desc. } *)
+  (*   des; auto. edestruct IMMyw; eauto.  *)
+  (* Qed.  *)
+    
+  Lemma stc_coherent (tc: trav_config) WF WFSC
+        (COH: tc_coherent G sc tc):
+    tc_coherent G sc (sim_trav_closure tc).
+  Proof.
+    apply tc_coherent_alt_implies_tc_coherent.
+    pose proof COH as COH'. apply tc_coherent_implies_tc_coherent_alt in COH'; auto.
+    inversion COH'.
+    rewrite stc_alt; auto.
+    forward eapply codom_I_rmw_empty as CIR; eauto.
+    destruct tc as [C I] eqn:TC. simpl in *. 
+    assert (sb^? ⨾ ⦗C⦘ ⊆ ⦗C⦘ ⨾ sb^? ⨾ ⦗C⦘) as COV_SB'.
+    { apply dom_rel_helper_in. 
+      rewrite crE, seq_union_l, dom_union. 
+      rewrite tc_sb_C. basic_solver. }
+    constructor; simpl. 
+    { etransitivity; [apply tc_init| ]. basic_solver. }
+    { admit. }
+    { rewrite id_union, seq_union_r, dom_union.
+      apply set_subset_union_l. split; [generalize tc_sb_C; basic_solver 10 | ].
+      unfold Cclos. simpl. rewrite id_union, seq_union_r, dom_union.
+      apply set_subset_union_l. split.
+      { apply set_subset_union_r. left.
+        replace C with (covered tc); [| by rewrite TC].
+        etransitivity.
+        2: { eapply dom_sb_W_rel_issued; eauto. rewrite TC. apply COH. }
+        rewrite TC. simpl. rewrite <- id_inter. apply dom_rel_mori. basic_solver. }
+      rewrite id_union, seq_union_l, codom_union.
+      rewrite id_union, seq_union_r, dom_union. 
+      rewrite CIR, eqv_empty, seq_false_r, dom_empty, set_union_empty_r. 
+      rewrite dom_rel_eqv_codom_rel. rewrite transp_seq, transp_eqv_rel. 
+      rewrite <- seqA, sb_invrmw_sbclos; auto.
+      rewrite COV_SB'. basic_solver. }
+    { rewrite set_inter_union_l. rewrite tc_W_C_in_I.
+      unfold Cclos, Iclos. simpl.
+      rewrite id_union, seq_union_l, codom_union, CIR.
+      basic_solver. }
+    { rewrite id_union, seq_union_r, dom_union, tc_rf_C.
+      unfold Cclos, Iclos. simpl.
+      rewrite !id_union, !seq_union_l, codom_union, CIR.
+      rewrite tc_I_in_W at 2. 
+      rewrite set_union_empty_r. rewrite wf_rmwD; auto.
+      do 3 rewrite codom_seq at 1. rewrite codom_eqv.
+      rewrite <- id_union. rewrite wf_rfD; auto. type_solver. }
+    { rewrite id_union, seq_union_r, dom_union, tc_sc_C.
+      unfold Cclos. simpl.
+      rewrite !id_union, !seq_union_l, codom_union, CIR, set_union_empty_r.
+      rewrite seq_union_r, dom_union. repeat (apply set_subset_union_l; split).
+      { basic_solver. }
+      { erewrite (wf_scD WFSC). rewrite tc_I_in_W at 1.
+        type_solver. }
+      erewrite (wf_scD WFSC). rewrite wf_rmwD at 1; auto.
+      do 3 rewrite codom_seq at 1. rewrite codom_eqv. type_solver. }
+    { admit. }
+    { admit. }
+    { rewrite !id_union, seq_union_r, dom_union, tc_fwbob_I.
+      unfold Iclos, Cclos. simpl.
+      rewrite fwbob_in_sb.
+      rewrite dom_rel_eqv_codom_rel. rewrite transp_seq, transp_eqv_rel.
+      rewrite <- seqA. rewrite sb_invrmw_sbclos; auto.
+      rewrite COV_SB'. basic_solver. }
+    { rewrite id_union, !seq_union_r, dom_union, tc_I_ar_rf_ppo_loc_I.
+      unfold Iclos. simpl.
+      unfold "ar". rewrite ct_end, seqA.
+      rewrite !seq_union_l.
+      arewrite (sc ⨾ ⦗codom_rel (⦗C⦘ ⨾ rmw)⦘ ⊆ ∅₂).
+      { rewrite (wf_scD WFSC), (wf_rmwD WF). type_solver. }
+      arewrite (rfe ⨾ ⦗codom_rel (⦗C⦘ ⨾ rmw)⦘ ⊆ ∅₂).
+      { rewrite wf_rfeD, wf_rmwD; auto. type_solver. }
+      rewrite ar_int_in_sb; auto.
+      arewrite (ppo ∩ same_loc ⊆ sb) at 2 by (generalize ppo_in_sb; basic_solver).
+      rewrite !union_false_l. rewrite !seq_union_r. rewrite dom_union.
+      repeat (apply set_subset_union_l; split).
+      { basic_solver. }
+      { rewrite <- !seqA. rewrite dom_rel_eqv_codom_rel.
+        rewrite transp_seq, transp_eqv_rel.
+        rewrite !seqA. rewrite <- seqA with (r3 := ⦗C⦘).
+        seq_rewrite sb_invrmw_sbclos; auto. 
+        rewrite COV_SB'. do 2 rewrite <- seqA. rewrite dom_seq.
+        rewrite rtE. rewrite seq_union_r, seq_union_l, dom_union.
+        apply set_subset_union_l. split.
+        { rewrite <- tc_W_C_in_I. basic_solver. }
+        (* TODO: need to restrict C to writes *)
+        admit. }
+      admit. }
+  Admitted. 
+        
   Lemma isim_trav_step_mon thread
         (C1 I1 C2 I2 C' I': actid -> Prop)
-        (* (C1 I1 C2 I2 C1' I1' C2' I2': actid -> Prop) *)
         (STEP: isim_trav_step G sc thread (mkTC C1 I1) (mkTC C2 I2))
         (* (MON_C: C1 ⊆₁ C1') (MON_I: C1 ⊆₁ C1') *)
         :
     (isim_trav_step G sc thread)^? (mkTC (C1 ∪₁ C') (I1 ∪₁ I'))
                    (mkTC (C2 ∪₁ C') (I2 ∪₁ I')).
-  Proof. 
+  Proof.
+    (* TODO: refactor *)
     inversion STEP; subst; simpl in *. 
     { destruct (classic ((C1 ∪₁ C') f)).
       { left. apply trav_config_eq_helper; simpl; basic_solver. }
@@ -198,6 +358,54 @@ Module SimTravClosure.
       2: { eapply itrav_step_more; [reflexivity| .. | apply H0].
            all: by apply same_tc_Symmetric. }
       inversion H0. destruct H. rewrite H2. basic_solver. }
+    { destruct (classic ((C1 ∪₁ C') r)).
+      { left. apply trav_config_eq_helper; simpl; basic_solver. }
+      right.
+      assert (C1 ∪₁ eq r ∪₁ C' ≡₁ C1 ∪₁ C' ∪₁ eq r) as C_ALT by basic_solver. 
+      erewrite trav_config_eq_helper'; [| simpl; by apply C_ALT | reflexivity].
+      simpl.
+      apply read_trav_step; auto. simpl.
+      erewrite trav_config_eq_helper'; [| simpl; by rewrite <- C_ALT | reflexivity].
+      simpl.
+      eapply itrav_step_mon_ext with (C' := C') (I' := I') in TS as [? | ?].
+      2: { eapply itrav_step_more; [reflexivity| .. | apply H0].
+           all: by apply same_tc_Symmetric. }
+      inversion H0. destruct H. rewrite H2. basic_solver. }
+    { destruct (classic ((I1 ∪₁ I') w)).
+      { left. apply trav_config_eq_helper; simpl; basic_solver. }
+      right.
+      assert (I1 ∪₁ eq w ∪₁ I' ≡₁ I1 ∪₁ I' ∪₁ eq w) as I_ALT by basic_solver. 
+      erewrite trav_config_eq_helper'; [| reflexivity| simpl; by apply I_ALT].
+      simpl.
+      apply rlx_write_promise_step; auto. simpl.
+      erewrite trav_config_eq_helper'; [| reflexivity| simpl; by rewrite <- I_ALT].
+      simpl.
+      eapply itrav_step_mon_ext with (C' := C') (I' := I') in TS as [? | ?].
+      2: { eapply itrav_step_more; [reflexivity| .. | apply H0].
+           all: by apply same_tc_Symmetric. }
+      inversion H0. destruct H. rewrite H2. basic_solver. }
+    { rename I2 into I1. 
+      destruct (classic ((C1 ∪₁ C') w)).
+      { left. apply trav_config_eq_helper; simpl; basic_solver. }
+      right.
+      assert (C1 ∪₁ eq w ∪₁ C' ≡₁ C1 ∪₁ C' ∪₁ eq w) as C_ALT by basic_solver. 
+      erewrite trav_config_eq_helper'; [| simpl; by apply C_ALT | reflexivity].
+      simpl.
+      apply rlx_write_cover_step; auto.
+      { simpl. red. tauto. } 
+      erewrite trav_config_eq_helper'; [| simpl; by rewrite <- C_ALT | reflexivity].
+      simpl.
+      eapply itrav_step_mon_ext with (C' := C') (I' := I') in TS as [? | ?].
+      2: { eapply itrav_step_more; [reflexivity| .. | apply H0].
+           all: by apply same_tc_Symmetric. }
+      inversion H0. destruct H. rewrite H2. basic_solver. }
+    { assert (~ C1 w) as NC1w.
+      { inversion TS2; red in H; desc; simpl in *; auto.
+        destruct NISS0. basic_solver. }
+      destruct (classic (C' w)) as [C'w | NC'w], (classic (I' w)) as [I'w | NI'w].
+      { left. apply trav_config_eq_helper; simpl; basic_solver. }
+      2: { 
+        (* TODO: so far it doesn't seem true *)
   Admitted.
 
   Lemma isim_trav_step_mon_tcu thread
@@ -234,7 +442,7 @@ Module SimTravClosure.
     eapply FUN; eauto.
   Qed.
 
-  Lemma trav_step_closures_isim WF CONS
+  Lemma trav_step_closures_isim WF WFSC CONS
         (tc tc': trav_config)
         (COH: tc_coherent G sc tc)
         (COH': tc_coherent G sc tc')
@@ -289,9 +497,9 @@ Module SimTravClosure.
              2: { by apply same_tc_Symmetric. }
              2: { split; auto. }   
              rewrite tcu_empty_l. rewrite <- Heqtc''. 
-             rewrite !stc_alt.
+             rewrite !stc_alt; auto. 
              rewrite tcu_assoc, tcu_symm with (tc2 := tc''), <- tcu_assoc.
-             apply isim_trav_step_mon_tcu.
+             apply isim_trav_step_mon_tcu; auto. 
              subst tc''. destruct tc as [C I], tc' as [C' I']. simpl in *.
              unfold trav_config_union. simpl.
              erewrite trav_config_eq_helper'; cycle 1. 
@@ -370,73 +578,11 @@ Module SimTravClosure.
           red. split.
           { split; auto. }
           repeat left. split; auto. basic_solver. }
+        
+        
   Admitted. 
              
 
-  Lemma trav_step_closures_isim WF
-        (tc tc': trav_config) 
-        (TRAV_STEP: trav_step G sc tc tc'):
-    (sim_trav_step G sc)^? (sim_trav_closure tc) (sim_trav_closure tc').
-  Proof.
-    assert (forall tc C1 I1 C2 I2
-              (COV: covered tc ≡₁ C1 ∪₁ C2)
-              (ISS: issued tc ≡₁ I1 ∪₁ I2),
-               tc = (mkTC C1 I1) ⊔ (mkTC C2 I2)) as TCU_HELPER.
-    { ins. unfold trav_config_union. apply trav_config_eq_helper; simpl; auto. }
-    red in TRAV_STEP. desc. red in TRAV_STEP. des.
-    { pose proof (lab_rwf lab e) as LABe. des.
-      { right. exists (tid e).
-
-        (* destruct tc as [C I], tc' as [C' I']. simpl in *. *)
-        remember (mkTC (eq e) ∅) as tc''. 
-        assert (tc' = tc ⊔ tc'') as TC'_UNION.
-        { subst tc''. apply trav_config_eq_helper; simpl; auto.
-          generalize ISSEQ. basic_solver. }
-        rewrite TC'_UNION, stc_tcu_distribute.
-                
-        assert (sim_trav_closure tc'' =
-                mkTC (eq e ∪₁ codom_rel (⦗eq e⦘ ⨾ rmw))
-                     (codom_rel (⦗eq e⦘ ⨾ rmw))) as TC''.
-        { apply trav_config_eq_helper; subst tc''; simpl.
-          { by rewrite !set_inter_empty_l, !set_union_empty_r. }
-          { rewrite !set_inter_empty_l, !set_union_empty_r, !set_union_empty_l.
-            rewrite set_inter_union_l. erewrite set_equiv_union.
-            3: { apply set_inter_absorb_r.
-                 rewrite wf_rmwD; auto; basic_solver. }
-            2: { apply set_subset_empty_r. type_solver. }
-            basic_solver. 
-          }
-        }        
-
-        rewrite TC''. rewrite !stc_alt. simpl.
-        remember ({| covered := Cclos tc; issued := Iclos tc |}) as tcc.
-
-        destruct (classic (dom_rel rmw e)) as [RMWr | NRMWr].
-        2: { rewrite tcu_assoc. rewrite tcu_symm with (tc1 := tcc), <- tcu_assoc.
-             eapply isim_trav_step_mon_tcu. 
-
-
-        
-        forward eapply eq_trans as TC''_UNION; [apply TC''| | ]. 
-        { eapply TCU_HELPER; simpl; [reflexivity| ]. 
-          symmetry. apply set_union_empty_l. }
-        rewrite <- TC'', TC''_UNION.
-
-         
-        
-
-
-        rewrite !stc_alt.
-        destruct tc as [C I], tc' as [C' I']. simpl in *.
-        (* unfold trav_config_union, Iclos, Cclos. *)
-        unfold trav_config_union. 
-        erewrite trav_config_eq_helper'. 
-        2: { simpl. rewrite COVEQ, ISSEQ. reflexivity. }
-        2: { simpl. rewrite ISSEQ, COVEQ. reflexivity. }
-        simpl. 
-
-        unfold Iclos, Cclos. simpl. 
-        fold Cclos. 
     
   Section Traversal.
     Variable (steps: nat -> t).
